json/Theorems/Utf8.v
@@ -47,6 +47,11 @@ Ltac to_bits byte :=
     end
   in 
   match type of byte with
+  | Utf8.codepoint =>
+      unfold Utf8.codepoint, Utf8.b4 in byte;
+      destruct byte as [[[[[b b4_1] b4_2] b4_3] b4_4] b4_5];
+      break_bit b4_1; break_bit b4_2; break_bit b4_3; break_bit b4_4; break_bit b4_5
+                         
   | Utf8.b6 =>
       unfold Utf8.b6 in byte; break_bit byte
   | Byte.byte =>
@@ -57,53 +62,148 @@ Ltac to_bits byte :=
       symmetry in eqn_name
   end.
 
-Lemma utf8_encode_correct : forall (c: codepoint) l,
-    l = utf8_encode_codepoint c  ->
-    (exists b1 b2 b3 b4 b5 b6 b7,
-        l = [ Byte.of_bits (b7, (b6, (b5, (b4, (b3, (b2, (b1, false))))))) ]
-        /\ c = (false, b4_zero, b4_zero, b4_zero, (false, b1, b2, b3), (b4, b5, b6, b7)) )
+Ltac no_overlongs :=
+  match goal with
+  | [ H: ?bit = true \/ ?b |- _] => destruct H; no_overlongs
+  | [ G: ?bit = true |- context[if ?bit then _ else _] ] => rewrite G
+  | |- context[if ?bit then _ else _] => destruct bit; [ no_overlongs | no_overlongs ]
+  end.
+
+Ltac crush_bits :=
+  repeat match goal with
+    | |- context[if ?bit then _ else _] => destruct bit
+    | _: context[if ?bit then _ else _ ] |- _ => destruct bit
+    end.
+
+Ltac no_overlongs2 :=
+  repeat match goal with
+    | [ H: ?bit = _ \/ ?b |- _] => destruct H
+    | [ G: ?bit = _ |- context[if ?bit then _ else _] ] => rewrite G
+    | [ F: context[if ?bit then _ else _] |- _] => destruct bit
+    | |- context[if ?bit then _ else _] => destruct bit
+    end.
+
+Theorem utf8_encode_codepoint_one_correct: forall (c: codepoint) b1 b2 b3 b4 b5 b6 b7,
+    utf8_encode_codepoint c = Some [ Byte.of_bits (b7, (b6, (b5, (b4, (b3, (b2, (b1, false))))))) ]
+    <-> c = (false, b4_zero, b4_zero, b4_zero, (false, b1, b2, b3), (b4, b5, b6, b7)).
+Proof.
+  split; intros.
+  - unfold utf8_encode_codepoint in H. to_bits c.
+    repeat match goal with
+           | [_: context[if ?bit then _ else _] |- _] => destruct bit
+           | [_: _ = _ |- _] => try discriminate
+           end. assert (forall T (a b: T), Some [a] = Some [b] -> a = b).
+    { intros. injection H0. auto. }
+    apply H0 in H.
+    apply (f_equal Byte.to_bits) in H. repeat rewrite Byte.to_bits_of_bits in H. inversion H. subst. reflexivity.
+  - subst. unfold utf8_encode_codepoint, b4_zero. reflexivity.
+Defined.
+
+Theorem utf8_encode_codepoint_two_correct: forall (c: codepoint) b1 b2 b3 b4 b5 b6 b7 b8 b9 b10 b11,
+    utf8_encode_codepoint c = Some [ Byte.of_bits (b5,  (b4,  (b3, (b2, (b1, (false,  (true, true)))))));
+                                     Byte.of_bits (b11, (b10, (b9, (b8, (b7, (b6, (false, true))))))) ]
+    <-> (c = (false, b4_zero, b4_zero, (false, b1, b2, b3), (b4, b5, b6, b7), (b8, b9, b10, b11))
+       /\ (b1 = true \/ b2 = true \/ b3 = true \/ b4 = true)).
+Proof.
+  split; intros.
+  - unfold utf8_encode_codepoint in H. to_bits c.
+    assert (forall T (a1 a2 b1 b2: T), Some [a1; a2] = Some [b1; b2] -> a1 = b1 /\ a2 = b2). { intros. injection H0. auto. }
+    repeat match goal with
+           | [_: context[if ?bit then _ else _] |- _] => destruct bit
+           | [_: _ = _ |- _] => try discriminate
+           end;
+    apply H0 in H as [H1 H2];
+    apply (f_equal Byte.to_bits) in H1, H2;
+      repeat (rewrite Byte.to_bits_of_bits in H1, H2); inversion H1; inversion H2; subst; split; auto.
+  - destruct H. subst. unfold utf8_encode_codepoint, b4_zero.
+    no_overlongs2; subst; reflexivity.
+Defined.
+
+Theorem utf8_encode_codepoint_three_correct: forall (c: codepoint) b1 b2 b3 b4 b5 b6 b7 b8 b9 b10 b11 b12 b13 b14 b15 b16,
+    utf8_encode_codepoint c = Some [ Byte.of_bits (b4,  (b3,  (b2,  (b1,  (false,   (true, (true, true)))))));
+                                     Byte.of_bits (b10, (b9,  (b8,  (b7,  (b6,  (b5,  (false, true)))))));
+                                     Byte.of_bits (b16, (b15, (b14, (b13, (b12, (b11, (false, true)))))))]
+    <-> (c = (false, b4_zero, (b1, b2, b3, b4), (b5, b6, b7, b8), (b9, b10, b11, b12), (b13, b14, b15, b16))
+             /\ (b1 = true \/ b2 = true \/ b3 = true \/ b4 = true \/ b5 = true) (* no overlong encodings *)
+             /\ (b1 = false \/ b2 = false \/ b3 = true \/ b4 = false \/ b5 = false)).
+Proof.
+  split; intros.
+  - unfold utf8_encode_codepoint in H. to_bits c.
+    assert (forall T (a1 a2 a3 b1 b2 b3: T), Some [a1; a2; a3] = Some [b1; b2; b3] -> a1 = b1 /\ a2 = b2 /\ a3 = b3). { intros. injection H0. auto. }
+    repeat match goal with
+           | [_: context[if ?bit then _ else _] |- _] => destruct bit
+           | [_: _ = _ |- _] => try discriminate
+           end;
+      apply H0 in H as [H1 [H2 H3]];
+      apply (f_equal Byte.to_bits) in H1, H2, H3;
+      repeat (rewrite Byte.to_bits_of_bits in H1, H2, H3); inversion H1; inversion H2; inversion H3; subst; repeat split; auto.
+  - destruct H as [H1 [H2 H3]]. unfold utf8_encode_codepoint, b4_zero in *. to_bits c. inversion_clear H1; subst.
+    no_overlongs2; subst; try discriminate; auto.
+Defined.
+
+Theorem utf8_encode_codepoint_four_correct: forall (c: codepoint) b1 b2 b3 b4 b5 b6 b7 b8 b9 b10 b11 b12 b13 b14 b15 b16 b17 b18 b19 b20 b21,
+    utf8_encode_codepoint c = Some [ Byte.of_bits (b3,  (b2,  (b1,  (false,   (true,  (true,   (true, true)))))));
+                                     Byte.of_bits (b9,  (b8,  (b7,  (b6,  (b5,  (b4,  (false, true)))))));
+                                     Byte.of_bits (b15, (b14, (b13, (b12, (b11, (b10, (false, true)))))));
+                                     Byte.of_bits (b21, (b20, (b19, (b18, (b17, (b16, (false, true))))))) ]
+    <-> (c = (b1, (b2, b3, b4, b5), (b6, b7, b8, b9), (b10, b11, b12, b13), (b14, b15, b16, b17), (b18, b19, b20, b21))
+             /\ (b1 = true \/ b2 = true \/ b3 = true \/ b4 = true \/ b5 = true)).
+Proof.
+  split; intros.
+  - unfold utf8_encode_codepoint in H. to_bits c.
+    assert (forall T (a1 a2 a3 a4 b1 b2 b3 b4: T), Some [a1; a2; a3; a4] = Some [b1; b2; b3; b4] -> a1 = b1 /\ a2 = b2 /\ a3 = b3 /\ a4 = b4). { intros. injection H0. auto. }
+    repeat match goal with
+           | [_: context[if ?bit then _ else _] |- _] => destruct bit
+           | [_: _ = _ |- _] => try discriminate
+           end;
+      apply H0 in H as [H1 [H2 [H3 H4]]];
+      apply (f_equal Byte.to_bits) in H1, H2, H3, H4;
+      repeat (rewrite Byte.to_bits_of_bits in H1, H2, H3, H4); inversion H1; inversion H2; inversion H3; inversion H4; subst; split; auto.
+  - destruct H as [H1 H2]. unfold utf8_encode_codepoint, b4_zero in *. to_bits c. inversion_clear H1; subst.
+    no_overlongs2; subst; try discriminate; auto.
+Defined.
+
+Lemma utf8_encode_codepoint_correct : forall (c: codepoint),
+    (utf8_encode_codepoint c = None)
+    \/ 
+      (exists b1 b2 b3 b4 b5 b6 b7,
+          utf8_encode_codepoint c = Some [ Byte.of_bits (b7, (b6, (b5, (b4, (b3, (b2, (b1, false))))))) ])
     \/ (exists b1 b2 b3 b4 b5 b6 b7 b8 b9 b10 b11,
-           l = [ Byte.of_bits (b5,  (b4,  (b3, (b2, (b1, (false,  (true, true)))))));
-                 Byte.of_bits (b11, (b10, (b9, (b8, (b7, (b6, (false, true))))))) ]
-           /\ c = (false, b4_zero, b4_zero, (false, b1, b2, b3), (b4, b5, b6, b7), (b8, b9, b10, b11))
-           /\ (b1 = true \/ b2 = true \/ b3 = true \/ b4 = true))
+           utf8_encode_codepoint c = Some [ Byte.of_bits (b5,  (b4,  (b3, (b2, (b1, (false,  (true, true)))))));
+                                            Byte.of_bits (b11, (b10, (b9, (b8, (b7, (b6, (false, true))))))) ]) 
     \/ (exists b1 b2 b3 b4 b5 b6 b7 b8 b9 b10 b11 b12 b13 b14 b15 b16,
-           l = [ Byte.of_bits (b4,  (b3,  (b2,  (b1,  (false,   (true, (true, true)))))));
-                 Byte.of_bits (b10, (b9,  (b8,  (b7,  (b6,  (b5,  (false, true)))))));
-                 Byte.of_bits (b16, (b15, (b14, (b13, (b12, (b11, (false, true)))))))]
-           /\ c = (false, b4_zero, (b1, b2, b3, b4), (b5, b6, b7, b8), (b9, b10, b11, b12), (b13, b14, b15, b16))
-           /\ (b1 = true \/ b2 = true \/ b3 = true \/ b4 = true \/ b5 = true))
+           utf8_encode_codepoint c = Some [ Byte.of_bits (b4,  (b3,  (b2,  (b1,  (false,   (true, (true, true)))))));
+                                            Byte.of_bits (b10, (b9,  (b8,  (b7,  (b6,  (b5,  (false, true)))))));
+                                            Byte.of_bits (b16, (b15, (b14, (b13, (b12, (b11, (false, true)))))))])
     \/ (exists b1 b2 b3 b4 b5 b6 b7 b8 b9 b10 b11 b12 b13 b14 b15 b16 b17 b18 b19 b20 b21,
-           l = [ Byte.of_bits (b3,  (b2,  (b1,  (false,   (true,  (true,   (true, true)))))));
-                 Byte.of_bits (b9,  (b8,  (b7,  (b6,  (b5,  (b4,  (false, true)))))));
-                 Byte.of_bits (b15, (b14, (b13, (b12, (b11, (b10, (false, true)))))));
-                 Byte.of_bits (b21, (b20, (b19, (b18, (b17, (b16, (false, true))))))) ]
-           /\ c = (b1, (b2, b3, b4, b5), (b6, b7, b8, b9), (b10, b11, b12, b13), (b14, b15, b16, b17), (b18, b19, b20, b21))
-           /\ (b1 = true \/ b2 = true \/ b3 = true \/ b4 = true \/ b5 = true)).
+           utf8_encode_codepoint c = Some [ Byte.of_bits (b3,  (b2,  (b1,  (false,   (true,  (true,   (true, true)))))));
+                                            Byte.of_bits (b9,  (b8,  (b7,  (b6,  (b5,  (b4,  (false, true)))))));
+                                            Byte.of_bits (b15, (b14, (b13, (b12, (b11, (b10, (false, true)))))));
+                                            Byte.of_bits (b21, (b20, (b19, (b18, (b17, (b16, (false, true))))))) ]). 
 Proof.
   intros.
-  destruct c as [[[[[b21 [[[b20 b19] b18] b17]]
-                      [[[b16 b15] b14] b13]]
-                     [[[b12 b11] b10] b9]]
-                    [[[b8 b7] b6] b5]]
-                   [[[b4 b3] b2] b1]].
-  unfold utf8_encode_codepoint in H.
-  repeat match goal with
-         | [_: l = if ?bit then [ _; _; _; _ ] else ?rest |- _] => destruct bit; [ right; right; right; repeat eexists; [ apply H | auto ] | ]
-         | [_: l = if ?bit then [ _; _; _ ] else ?rest |- _] => destruct bit; [ right; right; left; repeat eexists; [ apply H | auto ] |  ]
-         | [_: l = if ?bit then [ _; _ ] else ?rest |- _] => destruct bit; [ right; left; repeat eexists; [ apply H | auto ] | ]
-         end.
-  left. repeat eexists. apply H.
+  destruct (utf8_encode_codepoint c) eqn: utf8_enc_codepoint_c. 
+  to_bits c.
+  unfold utf8_encode_codepoint in utf8_enc_codepoint_c. symmetry in utf8_enc_codepoint_c.
+  no_overlongs2;
+    lazymatch type of utf8_enc_codepoint_c with
+    | context[Some [_]] => right; left; repeat eexists; apply utf8_enc_codepoint_c
+    | context[Some [_; _]]  => right; right; left; repeat eexists; apply utf8_enc_codepoint_c
+    | context[Some [_; _; _]]  => right; right; right; left; repeat eexists; apply utf8_enc_codepoint_c
+    | context[Some [_; _; _; _]]  => right; right; right; right; repeat eexists; apply utf8_enc_codepoint_c
+    | Some _ = None => discriminate
+    end. auto.
 Defined.
 
 Ltac for_all_valid_utf8_encodings c :=
-  let encodings := constr:(utf8_encode_correct c (utf8_encode_codepoint c) eq_refl) in
+  let encodings := constr:(utf8_encode_codepoint_correct c) in
   let rec f H :=
     match type of H with
     | exists bit : bool, _ => let b := fresh "b" in destruct H as [b _rest]; f _rest
     | ?a /\ ?b /\ ?c => destruct H as [eq [c_eq no_overlong]]
     | ?a /\ ?b => destruct H as [eq c_eq]
     | ?a \/ ?b => destruct H as [A | B]; [f A | f B]
+    | utf8_encode_codepoint c = _ => idtac
     end
   in f encodings.
 
@@ -127,11 +227,8 @@ Proof.
     to_bits byte;
     apply (f_equal Byte.of_bits) in byte_bits;
     rewrite Byte.of_bits_to_bits in byte_bits;
-    rewrite byte_bits;
-    repeat match goal with
-      | [ H: (if ?bit then _ else _) = _ |- _ ] => destruct bit
-      | [ |- (_ = _)] => try discriminate; inversion H; reflexivity
-      end.
+    rewrite byte_bits; 
+    crush_bits; try discriminate; inversion H; try reflexivity.
 Defined.
 
 Lemma enc_one_spec: forall b1 b2 b3 b4 b5 b6 b7, encoding_size_from_header (Byte.of_bits (b1, (b2, (b3, (b4, (b5, (b6, (b7, false)))))))) = Some (OneByte (b7, b6, b5, b4, b3, b2, b1)).
@@ -190,34 +287,35 @@ Proof.
   reflexivity.
 Defined.
 
-Theorem parse_codepoint_encode_correct : forall c rest, parse_codepoint ((utf8_encode_codepoint c) ++ rest)%list = Ok (c, rest).
+Theorem parse_codepoint_encode_correct : forall c bytes rest,
+    utf8_encode_codepoint c = Some bytes ->
+    parse_codepoint (bytes ++ rest)%list = Ok (c, rest).
 Proof.
-
-  Ltac no_overlongs :=
-    match goal with
-    | [ H: ?bit = true \/ ?b |- _] => destruct H; no_overlongs
-    | [ G: ?bit = true |- context[if ?bit then _ else _] ] => rewrite G; reflexivity
-    | |- context[if ?bit then _ else _] => destruct bit; [ reflexivity | no_overlongs ]
-    end.
-  
+  Opaque Byte.of_bits.
   intros.
-  for_all_valid_utf8_encodings c;
-    auto;
-    rewrite eq;
-    unfold parse_codepoint, parse_header, bind, app;
-    [ rewrite enc_one_spec | rewrite enc_two_spec | rewrite enc_three_spec | rewrite enc_four_spec];
-    rewrite c_eq;
-    repeat rewrite parse_continuation_spec;
-    try reflexivity;
-    unfold codepoint_range_to_codepoint, bind;
-    no_overlongs.
+  for_all_valid_utf8_encodings c; try (rewrite H in A; discriminate); [
+      apply utf8_encode_codepoint_one_correct in _rest as c_eq
+    | apply utf8_encode_codepoint_two_correct in _rest as G; destruct G as [c_eq no_overlongs]
+    | apply utf8_encode_codepoint_three_correct in _rest as G; destruct G as [c_eq [no_overlongs no_surrogates]]
+    | apply utf8_encode_codepoint_four_correct in _rest as G; destruct G as [c_eq no_overlongs]];
+    rewrite H in _rest;
+    injection _rest; intros; rewrite H0;
+    simpl; unfold parse_codepoint, parse_header, encoding_size_from_header, parse_continuation; rewrite Byte.to_bits_of_bits;
+    crush_bits;
+      subst; simpl;
+      repeat (rewrite parser_map_correct; simpl; rewrite Byte.to_bits_of_bits; simpl; rewrite Byte.to_bits_of_bits);
+      try reflexivity;
+      no_overlongs2; auto; subst; try discriminate.
 Defined.
 
-Lemma parse_single_codepoint_correct : forall c, parse_codepoint (utf8_encode_codepoint c) = Ok (c, []).
+Lemma parse_single_codepoint_correct : forall c bytes,
+    (utf8_encode_codepoint c) = Some bytes ->
+    parse_codepoint bytes = Ok (c, []).
 Proof.
   intros.
-  rewrite <- (List.app_nil_r (utf8_encode_codepoint c)).
-  apply (parse_codepoint_encode_correct c []).
+  apply parse_codepoint_encode_correct  with (rest := []) in H.
+  rewrite List.app_nil_r in H.
+  apply H.
 Defined.
 
 Ltac no_overlong_encoding Hyp :=
@@ -259,96 +357,113 @@ Proof.
       no_overlong_encoding H11; inversion H11; lia.
 Defined.
     
-Lemma many_codepoint_distributes : forall (c: codepoint) (cs: list codepoint),
-    many parse_codepoint (utf8_encode_codepoint c ++ concat (map utf8_encode_codepoint cs))%list =
-      let* (x, rest) := parse_codepoint (utf8_encode_codepoint c) in
-      let* (xs, rest) := many parse_codepoint (concat (map utf8_encode_codepoint cs)) in
-      Ok (x :: xs, rest).
+Theorem encode_decode_correct_strong : forall (unicode unicode_rest: unicode_str) bytes,
+  forall unicode_lesser,
+    (length unicode_lesser) <= (length unicode) -> 
+    utf8_encode unicode_lesser = Ok (bytes, unicode_rest) ->
+    utf8_decode bytes = Ok (unicode_lesser, []).
 Proof.
-  intros.
-  rewrite parse_single_codepoint_correct.
-  unfold many. simpl.
-  rewrite parse_codepoint_encode_correct.
-  unfold bind.
-  rewrite <- many_aux_saturation_aux with (n:= ( S ( S (Datatypes.length (utf8_encode_codepoint c ++ concat (map utf8_encode_codepoint cs))))));
-    [ reflexivity | apply parse_codepoint_strong_progress | | ];
-    for_all_valid_utf8_encodings c; rewrite eq; simpl; lia.
+  intros unicode.
+  induction unicode; intros.
+  - inversion H. rewrite length_zero_iff_nil in H2. subst. inversion H0; subst. unfold utf8_decode. simpl.
+  - destruct unicode_lesser as [| codepoint1 unicode_rest1] eqn:E_lesser.
+    + inversion H0. 
+    + simpl in H0.
+      destruct (utf8_encode_codepoint codepoint1) eqn:U_enc_codepoint1; [| discriminate H0].
+      destruct (utf8_encode unicode_rest1) as [[val2 rest2] | err] eqn:U_enc_unicode_rest1; [| discriminate H0].
+      inversion_clear H0. subst.
+      apply IHunicode with (unicode_lesser:= unicode_rest1) in U_enc_unicode_rest1; try (simpl in H; lia).
+      unfold utf8_decode, many. simpl.
+      apply parse_codepoint_encode_correct with (c := codepoint1) (rest := val2) in U_enc_codepoint1.
+      rewrite U_enc_codepoint1.
+      apply parse_codepoint_strong_progress in U_enc_codepoint1. unfold bind.
+      
 Defined.
 
-Theorem encode_decode_correct : forall u, utf8_decode (utf8_encode u) = Ok (u, []).
+Theorem encode_decode_correct : forall unicode unicode_rest bytes,
+    utf8_encode unicode = Ok (bytes, unicode_rest) ->
+    utf8_decode bytes = Ok (unicode, []).
 Proof.
   intros.
-  unfold utf8_encode, utf8_decode.
-  induction u; try reflexivity.
-  simpl.
-  rewrite many_codepoint_distributes.
-  rewrite parse_single_codepoint_correct.
-  rewrite IHu.
-  reflexivity.
+  apply encode_decode_correct_strong with (unicode := unicode) (unicode_rest := unicode_rest). lia.
+  apply H.
 Defined.
 
-Theorem decode_encode_correct_strong: forall (unicode: unicode_str) (bytes rest: list Byte.byte),
-    forall lesser, ((length lesser) <= (length bytes)) ->
-            (utf8_decode lesser = Ok (unicode, rest)) ->
-            lesser = List.app (utf8_encode unicode) rest.
+Theorem decode_encode_correct_strong: forall (bytes bytes_rest: list Byte.byte) (unicode: unicode_str),
+  forall bytes_lesser,
+    (length bytes_lesser) <= (length bytes) ->
+    utf8_decode bytes_lesser = Ok (unicode, bytes_rest) ->
+    utf8_encode unicode = Ok (bytes_lesser, []).
 Proof.
-  intros unicode bytes.
-  generalize dependent unicode.
-  destruct encoding_size_correct as [e1 [e2 [e3 e4]]].
-  induction bytes; intros unicode rest lesser enough_fuel IH_bytes.
-  - inversion enough_fuel. Search (List.length). rewrite length_zero_iff_nil in H0. subst. inversion IH_bytes. reflexivity.
-  - unfold utf8_decode, many in IH_bytes. simpl in IH_bytes.
-    destruct (parse_codepoint lesser) as [[val rest1] | err] eqn:Parse_lesser; [| inversion IH_bytes; reflexivity].
-    destruct lesser as [| byte1 bytes_rest1].
-    + inversion Parse_lesser; reflexivity.
-    + unfold parse_codepoint, parse_header in Parse_lesser.
-      destruct (encoding_size_from_header byte1) as [enc_size| ] eqn:Enc_byte1; simpl in Parse_lesser; [| inversion Parse_lesser; reflexivity].
-      destruct enc_size as [ [[[[[[b7 b6] b5] b4]b3] b2] b1]| [[[[b11 b10] b9] b8] b7] | [[[b16 b15] b14] b13] | [[b21 b20] b19] ] eqn:E_enc_size;
-        [ rewrite <- e1 in Enc_byte1 | rewrite <- e2 in Enc_byte1 |  rewrite <- e3 in Enc_byte1 | rewrite <- e4 in Enc_byte1 ];
-        subst;
-        unfold codepoint_range_to_codepoint, bind in Parse_lesser; simpl in Parse_lesser.
-      * inversion Parse_lesser. subst. clear Parse_lesser.
-        rewrite <- many_aux_saturation_aux with (n:= (S (Datatypes.length (Byte.of_bits (b1, (b2, (b3, (b4, (b5, (b6, (b7, false))))))) :: rest1)))) in IH_bytes; [ | apply parse_codepoint_strong_progress | simpl; lia |  simpl; lia ].
-        fold (many parse_codepoint rest1) in IH_bytes. fold (utf8_decode rest1) in IH_bytes.
-        destruct (utf8_decode rest1) as [[val rest2] | err] eqn:U_rest1; [| discriminate IH_bytes ].
-        inversion IH_bytes; apply IHbytes in U_rest1; subst. unfold utf8_encode, map. fold (map utf8_encode_codepoint). unfold concat. fold (concat (map utf8_encode_codepoint val)).
-        unfold utf8_encode_codepoint, b4_zero; reflexivity. simpl in enough_fuel. lia.
-      * destruct (parse_continuation bytes_rest1) as [[[[[[[b6 b5] b4] b3] b2] b1] bytes_rest2] | err] eqn: Parse_bytes_rest1; [ | discriminate Parse_lesser].
-        no_overlong_encoding Parse_lesser; inversion Parse_lesser; subst; clear Parse_lesser;
-        apply parse_continuation_strong_progress in Parse_bytes_rest1 as bytes_rest1_len;
-        rewrite <- many_aux_saturation_aux with (n:= S (S (Datatypes.length bytes_rest1))) in IH_bytes; try apply parse_codepoint_strong_progress; try (simpl; lia);
-        fold (many parse_codepoint rest1) in IH_bytes; fold (utf8_decode rest1) in IH_bytes;
-        destruct (utf8_decode rest1) as [[val rest2] | err] eqn:U_rest1; try discriminate IH_bytes;
-        inversion IH_bytes; apply IHbytes in U_rest1; subst; unfold utf8_encode, map; fold (map utf8_encode_codepoint); unfold concat; fold (concat (map utf8_encode_codepoint val));
-        unfold utf8_encode_codepoint, b4_zero; fold utf8_encode_codepoint;
-          destruct_parse_continuation; simpl in Parse_bytes_rest1; inversion Parse_bytes_rest1; subst;
-          try reflexivity; simpl in enough_fuel; lia. 
-      * destruct (parse_continuation bytes_rest1) as [[[[[[[b12 b11] b10] b9] b8] b7] bytes_rest2] | err] eqn: Parse_bytes_rest1; [ | discriminate Parse_lesser].
-        destruct (parse_continuation bytes_rest2) as [[[[[[[b6 b5] b4] b3] b2] b1] bytes_rest3] | err] eqn: Parse_bytes_rest2; [ | discriminate Parse_lesser].
-        no_overlong_encoding Parse_lesser; inversion Parse_lesser; subst; clear Parse_lesser;
-          apply parse_continuation_strong_progress in Parse_bytes_rest1 as bytes_rest1_len;
-          apply parse_continuation_strong_progress in Parse_bytes_rest2 as bytes_rest2_len;
-          rewrite <- many_aux_saturation_aux with (n:= S (S (Datatypes.length bytes_rest1))) in IH_bytes; try apply parse_codepoint_strong_progress; try (simpl; lia);
-          fold (many parse_codepoint rest1) in IH_bytes; fold (utf8_decode rest1) in IH_bytes; 
-          destruct (utf8_decode rest1) as [[val rest2] | err] eqn:U_rest1; try discriminate IH_bytes;
-          inversion IH_bytes; apply IHbytes in U_rest1; subst; unfold utf8_encode, map; fold (map utf8_encode_codepoint); unfold concat; fold (concat (map utf8_encode_codepoint val)); repeat destruct_parse_continuation;
-          unfold utf8_encode_codepoint, b4_zero; fold utf8_encode_codepoint; inversion Parse_bytes_rest2; inversion Parse_bytes_rest1; subst; try reflexivity; simpl in enough_fuel; lia.
-        * destruct (parse_continuation bytes_rest1) as [[[[[[[b18 b17] b16] b15] b14] b13] bytes_rest2] | err] eqn: Parse_bytes_rest1; [ | discriminate Parse_lesser].
-          destruct (parse_continuation bytes_rest2) as [[[[[[[b12 b11] b10] b9] b8] b7] bytes_rest3] | err] eqn: Parse_bytes_rest2; [ | discriminate Parse_lesser].
-          destruct (parse_continuation bytes_rest3) as [[[[[[[b6 b5] b4] b3] b2] b1] bytes_rest4] | err] eqn: Parse_bytes_rest3; [ | discriminate Parse_lesser].
-          apply parse_continuation_strong_progress in Parse_bytes_rest1 as bytes_rest1_len;
-            apply parse_continuation_strong_progress in Parse_bytes_rest2 as bytes_rest2_len;
-            apply parse_continuation_strong_progress in Parse_bytes_rest3 as bytes_rest3_len;
-          rewrite <- many_aux_saturation_aux with (n:= S (S (Datatypes.length bytes_rest1))) in IH_bytes;
-            [ | apply parse_codepoint_strong_progress | | ];
-            try (no_overlong_encoding Parse_lesser; inversion Parse_lesser; simpl; simpl in enough_fuel; subst; lia).
-          fold (many parse_codepoint rest1) in IH_bytes; fold (utf8_decode rest1) in IH_bytes.
-          destruct (utf8_decode rest1) as [[val2 rest2] | err] eqn:U_rest1; try discriminate IH_bytes.
-          repeat destruct_parse_continuation. inversion Parse_bytes_rest1; inversion Parse_bytes_rest2; inversion Parse_bytes_rest3; subst.
-          inversion IH_bytes; apply IHbytes in U_rest1;
-            no_overlong_encoding Parse_lesser; inversion Parse_lesser; subst; clear Parse_lesser; subst;
-            try (simpl in *; lia);
-            unfold utf8_encode, map; fold (map utf8_encode_codepoint); unfold concat; fold (concat (map utf8_encode_codepoint val2)); try reflexivity.
+  intros bytes.
+  induction bytes; intros.
+  - inversion H. rewrite length_zero_iff_nil in H2. subst. inversion H0. split; reflexivity.
+  - destruct bytes_lesser as [| bytes1 bytes_rest1] eqn:E_lesser.
+    + inversion H0; reflexivity.
+    + unfold utf8_decode, many in H0. simpl in H0.
+      destruct (parse_codepoint (bytes1 :: bytes_rest1)) as [[bytes2 bytes_rest2] | err] eqn:Parse_bytes1.
+      2: { 
+           
+      destruct (parse_codepoint bytes_rest2) as [[bytes3 bytes_rest3] | err] eqn:Parse_bytes_rest2.
+      
+    
+    
+  (* generalize dependent unicode. *)
+  (* destruct encoding_size_correct as [e1 [e2 [e3 e4]]]. *)
+  (* induction bytes; intros unicode rest lesser enough_fuel IH_bytes. *)
+  (* - inversion enough_fuel. rewrite length_zero_iff_nil in H0. subst. inversion IH_bytes. reflexivity. *)
+  (* - unfold utf8_decode, many in IH_bytes. simpl in IH_bytes. *)
+  (*   destruct (parse_codepoint lesser) as [[val rest1] | err] eqn:Parse_lesser; [| inversion IH_bytes; reflexivity]. *)
+  (*   destruct lesser as [| byte1 bytes_rest1]. *)
+  (*   + inversion Parse_lesser; reflexivity. *)
+  (*   + unfold parse_codepoint, parse_header in Parse_lesser. *)
+  (*     destruct (encoding_size_from_header byte1) as [enc_size| ] eqn:Enc_byte1; simpl in Parse_lesser; [| inversion Parse_lesser; reflexivity]. *)
+  (*     destruct enc_size as [ [[[[[[b7 b6] b5] b4]b3] b2] b1]| [[[[b11 b10] b9] b8] b7] | [[[b16 b15] b14] b13] | [[b21 b20] b19] ] eqn:E_enc_size; *)
+  (*       [ rewrite <- e1 in Enc_byte1 | rewrite <- e2 in Enc_byte1 |  rewrite <- e3 in Enc_byte1 | rewrite <- e4 in Enc_byte1 ]; *)
+  (*       subst; *)
+  (*       unfold codepoint_range_to_codepoint, bind in Parse_lesser; simpl in Parse_lesser. *)
+  (*     * inversion Parse_lesser. subst. clear Parse_lesser. *)
+  (*       rewrite <- many_aux_saturation_aux with (n:= (S (Datatypes.length (Byte.of_bits (b1, (b2, (b3, (b4, (b5, (b6, (b7, false))))))) :: rest1)))) in IH_bytes; [ | apply parse_codepoint_strong_progress | simpl; lia |  simpl; lia ]. *)
+  (*       fold (many parse_codepoint rest1) in IH_bytes. fold (utf8_decode rest1) in IH_bytes. *)
+  (*       destruct (utf8_decode rest1) as [[val rest2] | err] eqn:U_rest1; [| discriminate IH_bytes ]. *)
+  (*       inversion IH_bytes; apply IHbytes in U_rest1; subst. unfold utf8_encode, map. fold (map utf8_encode_codepoint). unfold concat. fold (concat (map utf8_encode_codepoint val)). *)
+  (*       unfold utf8_encode_codepoint, b4_zero; reflexivity. simpl in enough_fuel. lia. *)
+  (*     * destruct (parse_continuation bytes_rest1) as [[[[[[[b6 b5] b4] b3] b2] b1] bytes_rest2] | err] eqn: Parse_bytes_rest1; [ | discriminate Parse_lesser]. *)
+  (*       no_overlong_encoding Parse_lesser; inversion Parse_lesser; subst; clear Parse_lesser; *)
+  (*       apply parse_continuation_strong_progress in Parse_bytes_rest1 as bytes_rest1_len; *)
+  (*       rewrite <- many_aux_saturation_aux with (n:= S (S (Datatypes.length bytes_rest1))) in IH_bytes; try apply parse_codepoint_strong_progress; try (simpl; lia); *)
+  (*       fold (many parse_codepoint rest1) in IH_bytes; fold (utf8_decode rest1) in IH_bytes; *)
+  (*       destruct (utf8_decode rest1) as [[val rest2] | err] eqn:U_rest1; try discriminate IH_bytes; *)
+  (*       inversion IH_bytes; apply IHbytes in U_rest1; subst; unfold utf8_encode, map; fold (map utf8_encode_codepoint); unfold concat; fold (concat (map utf8_encode_codepoint val)); *)
+  (*       unfold utf8_encode_codepoint, b4_zero; fold utf8_encode_codepoint; *)
+  (*         destruct_parse_continuation; simpl in Parse_bytes_rest1; inversion Parse_bytes_rest1; subst; *)
+  (*         try reflexivity; simpl in enough_fuel; lia.  *)
+  (*     * destruct (parse_continuation bytes_rest1) as [[[[[[[b12 b11] b10] b9] b8] b7] bytes_rest2] | err] eqn: Parse_bytes_rest1; [ | discriminate Parse_lesser]. *)
+  (*       destruct (parse_continuation bytes_rest2) as [[[[[[[b6 b5] b4] b3] b2] b1] bytes_rest3] | err] eqn: Parse_bytes_rest2; [ | discriminate Parse_lesser]. *)
+  (*       no_overlong_encoding Parse_lesser; inversion Parse_lesser; subst; clear Parse_lesser; *)
+  (*         apply parse_continuation_strong_progress in Parse_bytes_rest1 as bytes_rest1_len; *)
+  (*         apply parse_continuation_strong_progress in Parse_bytes_rest2 as bytes_rest2_len; *)
+  (*         rewrite <- many_aux_saturation_aux with (n:= S (S (Datatypes.length bytes_rest1))) in IH_bytes; try apply parse_codepoint_strong_progress; try (simpl; lia); *)
+  (*         fold (many parse_codepoint rest1) in IH_bytes; fold (utf8_decode rest1) in IH_bytes;  *)
+  (*         destruct (utf8_decode rest1) as [[val rest2] | err] eqn:U_rest1; try discriminate IH_bytes; *)
+  (*         inversion IH_bytes; apply IHbytes in U_rest1; subst; unfold utf8_encode, map; fold (map utf8_encode_codepoint); unfold concat; fold (concat (map utf8_encode_codepoint val)); repeat destruct_parse_continuation; *)
+  (*         unfold utf8_encode_codepoint, b4_zero; fold utf8_encode_codepoint; inversion Parse_bytes_rest2; inversion Parse_bytes_rest1; subst; try reflexivity; simpl in enough_fuel; lia. *)
+  (*       * destruct (parse_continuation bytes_rest1) as [[[[[[[b18 b17] b16] b15] b14] b13] bytes_rest2] | err] eqn: Parse_bytes_rest1; [ | discriminate Parse_lesser]. *)
+  (*         destruct (parse_continuation bytes_rest2) as [[[[[[[b12 b11] b10] b9] b8] b7] bytes_rest3] | err] eqn: Parse_bytes_rest2; [ | discriminate Parse_lesser]. *)
+  (*         destruct (parse_continuation bytes_rest3) as [[[[[[[b6 b5] b4] b3] b2] b1] bytes_rest4] | err] eqn: Parse_bytes_rest3; [ | discriminate Parse_lesser]. *)
+  (*         apply parse_continuation_strong_progress in Parse_bytes_rest1 as bytes_rest1_len; *)
+  (*           apply parse_continuation_strong_progress in Parse_bytes_rest2 as bytes_rest2_len; *)
+  (*           apply parse_continuation_strong_progress in Parse_bytes_rest3 as bytes_rest3_len; *)
+  (*         rewrite <- many_aux_saturation_aux with (n:= S (S (Datatypes.length bytes_rest1))) in IH_bytes; *)
+  (*           [ | apply parse_codepoint_strong_progress | | ]; *)
+  (*           try (no_overlong_encoding Parse_lesser; inversion Parse_lesser; simpl; simpl in enough_fuel; subst; lia). *)
+  (*         fold (many parse_codepoint rest1) in IH_bytes; fold (utf8_decode rest1) in IH_bytes. *)
+  (*         destruct (utf8_decode rest1) as [[val2 rest2] | err] eqn:U_rest1; try discriminate IH_bytes. *)
+  (*         repeat destruct_parse_continuation. inversion Parse_bytes_rest1; inversion Parse_bytes_rest2; inversion Parse_bytes_rest3; subst. *)
+  (*         inversion IH_bytes; apply IHbytes in U_rest1; *)
+  (*           no_overlong_encoding Parse_lesser; inversion Parse_lesser; subst; clear Parse_lesser; subst; *)
+  (*           try (simpl in *; lia); *)
+  (*           unfold utf8_encode, map; fold (map utf8_encode_codepoint); unfold concat; fold (concat (map utf8_encode_codepoint val2)); try reflexivity. *)
 Defined.
 
 Theorem decode_encode_correct: forall (unicode: unicode_str) (bytes rest: list Byte.byte),
